added fractions

Test/civl/inductive-sequentialization/Easy-PC2-new.bpl
@@ -2,30 +2,37 @@
 // RUN: %diff "%s.expect" "%t"
 
 type Pid = int;
-type  Cid = int;
 type Duration = int;
+type ReqId;
 
 
 datatype Vote { YES(), NO(), NULL() }
 
 datatype Decision { COMMIT(), ABORT(), NONE() }
 
-type ReqId;
 
-datatype Request { Request(id: ReqId, duration: Duration)}
 
-const n:int;
-axiom n > 0;
+datatype Request { Request(id: ReqId, duration: Duration )}
+
+type ParticipantPiece = Fraction ReqId Pid;
+
+// 1, dur 3
+// 1, dur 6 
+
+// only reqId should be linear
+
+const NumParticipants:int;
+axiom NumParticipants > 0;
 
 var {:layer 0,1} locked_requests: [Pid](Set Request);
 var {:layer 0,1} participant_votes: [Pid][Request]Vote;
 var {:layer 0,1} committed_requests: (Set Request);
 
-function {:inline} Init(req: Request, participant_votes: [Pid][Request]Vote) : bool
-{
-//   participant_votes == (lambda p:Pid :: (lambda r:Request  :: NULL())) 
-  (forall p: Pid :: participant_votes[p][req] == NULL())
-}
+// function {:inline} Init(req: Request, participant_votes: [Pid][Request]Vote) : bool
+// {
+// //   participant_votes == (lambda p:Pid :: (lambda r:Request  :: NULL())) 
+//   (forall p: Pid :: participant_votes[p][req] == NULL())
+// }
 
 function {:inline} NoOverlap(req_set: (Set Request), d: Duration) : bool
 {
@@ -61,30 +68,71 @@ invariant !(exists req: Request, pid: Pid :: Set_Contains(committed_requests, re
 yield invariant {:layer 1} YieldTrue();
 invariant true;
 
-yield procedure {:layer 1} coordinator( cid: Cid,  req: Request)
+yield invariant {:layer 1} YieldVoting({:linear} pid: One ParticipantPiece, req: Request);
+invariant !(exists req0:Request :: Set_Contains(locked_requests[pid->val->id], req0) && req0->id == req->id);
+invariant participant_votes[pid->val->id][req] == NULL();
+
+// function {:inline} Init2(pids:[Pid]bool) : bool
+// {
+//   pids == MapConst(true)
+// }
+
+// yield invariant {:layer 1} YieldInit2({:linear} pids: Set Pid);
+// invariant Init2(pids->val);
+
+function {:inline} ParticipantIds(): Set Pid {
+    Set((lambda {:pool "P1"} x: int :: 1 <= x && x <= NumParticipants))
+}
+
+function {:inline} JParticipantIds(j: int): Set Pid {
+    Set((lambda {:pool "P1"} x: int :: j <= x && x <= NumParticipants))
+}
+
+function {:inline} AllParticipantPieces(r: ReqId): Set ParticipantPiece {
+    Set((lambda {:pool "P2"} x: ParticipantPiece :: x->val == r && x->ids == ParticipantIds() && Set_Contains(x->ids, x->id)))
+}
+
+function {:inline} JParticipantPieces(r: ReqId, j: int): Set ParticipantPiece {
+    Set((lambda {:pool "P2"} x: ParticipantPiece :: x->val == r && x->ids == ParticipantIds() && Set_Contains(JParticipantIds(j), x->id)))
+}
+
+yield procedure {:layer 1} coordinator({:linear_in} reqId: One ReqId, duration: Duration)
 // refines not_skip;
 // requires call YieldInit(req);
-// requires {:layer 1} (forall p: Pid :: participant_votes[p][req] == NULL());
+// requires {:layer 1} (forall p: Pid :: old(participant_votes)[p][req] == NULL());
+// requires call YieldInit2(pids);
 requires call YieldBig();
+// requires pids  == lambda .. are from 1 to n;
 {
    var i: int;
    var j: int;
    var d: Decision;
    var v: Vote;
+   var {:linear} pids: Set ParticipantPiece;
+   var {:linear} pid: One ParticipantPiece;
+   var {:linear} reqId': One ReqId;
+   
+
+   reqId' := reqId;
    d := COMMIT();
    j := 1;
-   while (j <= n)
+   call pids := One_To_Fractions(reqId', ParticipantIds());
+//    assert {:layer 1} pids == AllParticipantPieces(reqId'->val);
+   while (j <= NumParticipants)
+   invariant {:layer 1} 1 <= j && j <= NumParticipants + 1;
+   invariant {:layer 1} pids == JParticipantPieces(reqId'->val, j);
    {
-    async call voting0(req, i);
+    call pid := One_Get(pids, (Fraction(reqId'->val, j, ParticipantIds())));
+    async call voting0(Request(reqId'->val, duration), pid);
     j := j + 1;
    }
 
    call YieldBig();
    
    i := 1;
-   while (i <= n)
+   while (i <= NumParticipants)
    {
-    call v := receive_vote(i, req);
+    call v := receive_vote(i, Request(reqId'->val, duration));
     if (v == NO())
     {
     d := ABORT();
@@ -101,38 +149,41 @@ requires call YieldBig();
         // committed => locked
         // locked has no overlaps
         assume false;
-        assert {:layer 1} !(exists req1: Request :: req1->id != req->id && req1->duration == req->duration && Set_Contains(committed_requests, req1));
-        call add_to_committed_requests(req);
+        // assert {:layer 1} !(exists req1: Request :: req1->id != req->id && req1->duration == req->duration && Set_Contains(committed_requests, req1));
+        call add_to_committed_requests(Request(reqId'->val, duration));
    }
 }
 
-async action {:layer 1} voting( req: Request,  pid: Pid)
+async action {:layer 1} voting(req: Request, {:linear_in} pid: One ParticipantPiece)
 modifies locked_requests, participant_votes;
-asserts !(exists req0:Request :: Set_Contains(locked_requests[pid], req0) && req0->id == req->id);
-asserts participant_votes[pid][req] == NULL();
+// asserts !(exists req0:Request :: Set_Contains(locked_requests[pid], req0) && req0->id == req->id);
+// asserts participant_votes[pid][req] == NULL();
 {
-    // assert !(exists req0:Request :: Set_Contains(locked_requests[pid], req0) && req0->id == req->id);
-    // assert participant_votes[pid][req] == NULL();
+    assert !(exists req0:Request :: Set_Contains(locked_requests[pid->val->id], req0) && req0->id == req->id);
+    assert participant_votes[pid->val->id][req] == NULL();
     if (*) {
-        participant_votes[pid][req] := NO();
+        participant_votes[pid->val->id][req] := NO();
         return;
     }
     else {
-        if (NoOverlap(locked_requests[pid], req->duration)) {
-            locked_requests[pid] := Set_Add(locked_requests[pid], req);
-            participant_votes[pid][req] := YES();
+        if (NoOverlap(locked_requests[pid->val->id], req->duration)) {
+            locked_requests[pid->val->id] := Set_Add(locked_requests[pid->val->id], req);
+            participant_votes[pid->val->id][req] := YES();
         }
         else {
-            participant_votes[pid][req] := NO();
+            participant_votes[pid->val->id][req] := NO();
         }
     }
 }
-yield procedure {:layer 0} voting1(req: Request, pid: Pid);
+yield procedure {:layer 0} voting1(req: Request, {:linear_in} pid: One ParticipantPiece);
 refines voting;
 
-yield procedure {:layer 1} voting0(req: Request, pid: Pid)
+yield procedure {:layer 1} voting0(req: Request, {:linear_in}  pid: One ParticipantPiece)
 requires call YieldBig();
+requires call YieldVoting(pid, req);
 {
+    // assert {:layer 1} !(exists req0:Request :: Set_Contains((locked_requests)[pid], req0) && req0->id == req->id);
+    // assert {:layer 1} (participant_votes)[pid][req] == NULL();
     call voting1(req, pid);
 }
 
@@ -146,17 +197,17 @@ asserts !(exists req1: Request :: req1->id != req->id && req1->duration == req->
 yield procedure {:layer 0} add_to_committed_requests( req: Request);
 refines ADD_TO_COMMITTED_REQUESTS;
 
-right action {:layer 1} RECEIVE_VOTE( pid: Pid, req: Request) returns (v: Vote)
+right action {:layer 1} RECEIVE_VOTE(pid: Pid, req: Request) returns (v: Vote)
 {
    assume participant_votes[pid][req] != NULL();
    v := participant_votes[pid][req];
 }
-yield procedure {:layer 0} receive_vote( pid: Pid,  req: Request) returns (v: Vote);
+yield procedure {:layer 0} receive_vote(pid: Pid,  req: Request) returns (v: Vote);
 refines RECEIVE_VOTE;
 
 action {:layer 1} WAIT_FOR_PARTICIPANT_VOTE( req: Request)
 {
-      assume (forall pid: Pid :: (1 <= pid && pid <= n) ==> participant_votes[pid][req] != NULL());
+      assume (forall pid: Pid :: (1 <= pid && pid <= NumParticipants) ==> participant_votes[pid][req] != NULL());
 }
 yield procedure {:layer 0} wait_for_participant_vote( req: Request); 
 refines WAIT_FOR_PARTICIPANT_VOTE;
